src/num/theories/arithmeticScript.sml
@@ -82,30 +82,30 @@ val _ = new_definition(
 
 val _ = add_numeral_form (#"n", NONE);
 
+val _ = set_fixity "-" (Infixl 500);
 val SUB = new_recursive_definition
    {name = "SUB",
     rec_axiom = num_Axiom,
-    def = --`($- 0 m = 0) /\
-             ($- (SUC m) n = ((m < n) => 0 | SUC($- m n)))`--};
-val _ = set_fixity "-" (Infixl 500);
+    def = --`(0 - m = 0) /\
+             (SUC m - n = if m < n then 0 else SUC(m - n))`--};
 
+val _ = set_fixity "*" (Infixl 600);
 val MULT = new_recursive_definition
    {name = "MULT",
     rec_axiom = num_Axiom,
-    def = --`($* 0 n = 0) /\
-             ($* (SUC m) n = ($* m n) + n)`--};
-val _ = set_fixity "*" (Infixl 600);
+    def = --`(0 * n = 0) /\
+             (SUC m * n = (m * n) + n)`--};
+
 
 val EXP = new_recursive_definition
    {name = "EXP",
     rec_axiom = num_Axiom,
     def = --`($EXP m 0 = 1) /\
              ($EXP m (SUC n) = m * ($EXP m n))`--};
+
 val _ = set_fixity "EXP" (Infixr 700);
-
-val _ = add_infix("**", 700, HOLgrammars.RIGHT);
+val _ = add_infix("**", 700, HOLgrammars.RIGHT); 
 val _ = overload_on ("**", Term`$EXP`);
-
 
 val GREATER_DEF = new_infixr_definition
   ("GREATER_DEF", --`$> m n = n < m`--,   450);
@@ -2983,161 +2983,6 @@ val EXP2_LT = store_thm
           REWRITE_TAC [DOUBLE_LT]
           THEN REWRITE_TAC [TWO, ADD_0, LESS_MULT_MONO]]);
 
-(* ----------------------------------------------------------------------
-    least n satisfying P
-   ---------------------------------------------------------------------- *)
-
-val ITERATION = prove(
-  ``!P g. ?f. !x. f x = if P x then x else f (g x)``,
-  REPEAT GEN_TAC THEN
-  Q.EXISTS_TAC `\x. if ?n. P (FUNPOW g n x) then
-                      FUNPOW g (@n. P (FUNPOW g n x) /\
-                                    !m.  m < n ==> ~P (FUNPOW g m x)) x
-                    else ARB` THEN BETA_TAC THEN
-  GEN_TAC THEN COND_CASES_TAC THENL [
-    POP_ASSUM STRIP_ASSUME_TAC THEN
-    COND_CASES_TAC THENL [
-      SELECT_ELIM_TAC THEN CONJ_TAC THENL [
-        Q.EXISTS_TAC `0` THEN
-        ASM_REWRITE_TAC [FUNPOW, NOT_LESS_0],
-        Q.X_GEN_TAC `m` THEN REPEAT STRIP_TAC THEN
-        Q.SUBGOAL_THEN `m = 0` (fn th => REWRITE_TAC [th, FUNPOW]) THEN
-        Q.SPEC_THEN `m` (REPEAT_TCL STRIP_THM_THEN SUBST_ALL_TAC)
-                    num_CASES THEN
-        REWRITE_TAC [] THEN
-        FIRST_X_ASSUM (Q.SPEC_THEN `0` MP_TAC) THEN
-        ASM_REWRITE_TAC [FUNPOW, LESS_0]
-      ],
-      SELECT_ELIM_TAC THEN
-      CONJ_TAC THENL [
-        Q.SPEC_THEN `\n. P (FUNPOW g n x)` (IMP_RES_TAC o BETA_RULE) WOP THEN
-        PROVE_TAC [],
-        Q.X_GEN_TAC `m` THEN REPEAT STRIP_TAC THEN
-        Q.SUBGOAL_THEN `?p. m = SUC p` (CHOOSE_THEN SUBST_ALL_TAC) THENL [
-          Q.SPEC_THEN `m` (REPEAT_TCL STRIP_THM_THEN SUBST_ALL_TAC)
-                      num_CASES THEN
-          FULL_SIMP_TAC bool_ss [FUNPOW] THEN PROVE_TAC [],
-          ALL_TAC
-        ] THEN
-        FULL_SIMP_TAC bool_ss [FUNPOW] THEN
-        Q.SUBGOAL_THEN `?n. P (FUNPOW g n (g x))`
-                       (fn th => REWRITE_TAC [th]) THEN1 PROVE_TAC [] THEN
-        POP_ASSUM (Q.SPEC_THEN `SUC m` (ASSUME_TAC o GEN_ALL o
-                                        SIMP_RULE bool_ss [FUNPOW,
-                                                           LESS_MONO_EQ])) THEN
-        SELECT_ELIM_TAC THEN CONJ_TAC THENL [
-          PROVE_TAC [],
-          Q.X_GEN_TAC `m` THEN REPEAT STRIP_TAC THEN
-          PROVE_TAC [LESS_LESS_CASES]
-        ]
-      ]
-    ],
-    POP_ASSUM (ASSUME_TAC o SIMP_RULE bool_ss []) THEN
-    FIRST_ASSUM (ASSUME_TAC o SIMP_RULE bool_ss [FUNPOW] o
-                 GEN_ALL o SPEC ``SUC n``) THEN
-    ASM_REWRITE_TAC [] THEN PROVE_TAC [FUNPOW]
-  ]);
-
-val cond_lemma = prove(
-  ``(if ~p then q else r) = (if p then r else q)``,
-  Q.ASM_CASES_TAC `p` THEN ASM_REWRITE_TAC []);
-
-val o_THM = combinTheory.o_THM
-
-(* WHILE = |- !P g x. WHILE P g x = if P x then WHILE P g (g x) else x *)
-
-val WHILE = new_specification (
-  "WHILE", ["WHILE"],
-  (CONV_RULE (BINDER_CONV SKOLEM_CONV THENC SKOLEM_CONV) o GEN_ALL o
-   REWRITE_RULE [o_THM, cond_lemma] o
-   SPEC ``$~ o P : 'a -> bool``) ITERATION);
-
-val LEAST_DEF = new_definition(
-  "LEAST_DEF",
-  ``LEAST P = WHILE ($~ o P) SUC 0``);
-
-val _ = set_fixity "LEAST" Binder;
-
-val LEAST_INTRO = store_thm(
-  "LEAST_INTRO",
-  ``!P x. P x ==> P ($LEAST P)``,
-  GEN_TAC THEN SIMP_TAC (srw_ss()) [LEAST_DEF] THEN
-  Q_TAC SUFF_TAC `!m n. P (m + n) ==> P (WHILE ($~ o P) SUC n)`
-  THENL [
-    SRW_TAC [][] THEN
-    FIRST_X_ASSUM (Q.SPECL_THEN [`x`,`0`] MP_TAC) THEN
-    ASM_SIMP_TAC bool_ss [ADD_CLAUSES],
-    ALL_TAC
-  ] THEN
-  INDUCT_TAC THENL [
-    ONCE_REWRITE_TAC [WHILE] THEN
-    ASM_SIMP_TAC bool_ss [ADD_CLAUSES, o_THM],
-    ONCE_REWRITE_TAC [WHILE] THEN
-    SRW_TAC [][ADD_CLAUSES] THEN
-    FIRST_X_ASSUM MATCH_MP_TAC THEN
-    ASM_SIMP_TAC bool_ss [ADD_CLAUSES]
-  ]);
-
-val LESS_LEAST = store_thm(
-  "LESS_LEAST",
-  ``!P m. m < $LEAST P ==> ~ P m``,
-  GEN_TAC THEN
-  Q.ASM_CASES_TAC `?x. P x` THENL [
-    POP_ASSUM STRIP_ASSUME_TAC THEN
-    REWRITE_TAC [LEAST_DEF] THEN
-    Q_TAC SUFF_TAC `!y n. n + y < WHILE ($~ o P) SUC n ==> ~P(n + y)` THENL [
-      STRIP_TAC THEN GEN_TAC THEN
-      POP_ASSUM (Q.SPECL_THEN [`m`, `0`] MP_TAC) THEN
-      SIMP_TAC bool_ss [ADD_CLAUSES],
-      ALL_TAC
-    ] THEN
-    INDUCT_TAC THENL [
-      ONCE_REWRITE_TAC [WHILE] THEN SRW_TAC [][LESS_REFL, ADD_CLAUSES],
-      GEN_TAC THEN
-      Q.SUBGOAL_THEN `n + SUC y = SUC n + y` SUBST_ALL_TAC THEN1
-        SRW_TAC [][ADD_CLAUSES] THEN
-      STRIP_TAC THEN FIRST_X_ASSUM MATCH_MP_TAC THEN
-      RULE_ASSUM_TAC (ONCE_REWRITE_RULE [WHILE]) THEN
-      Q.ASM_CASES_TAC `P n` THEN FULL_SIMP_TAC (srw_ss()) [] THEN
-      Q.SUBGOAL_THEN `SUC n + y = n + SUC y` SUBST_ALL_TAC THEN1
-        SRW_TAC [][ADD_CLAUSES] THEN
-      PROVE_TAC [LESS_ADD_SUC, LESS_TRANS, LESS_REFL]
-    ],
-    PROVE_TAC []
-  ]);
-
-val FULL_LEAST_INTRO = store_thm(
-  "FULL_LEAST_INTRO",
-  ``!x. P x ==> P ($LEAST P) /\ $LEAST P <= x``,
-  PROVE_TAC [LEAST_INTRO, NOT_LESS, LESS_LEAST]);
-
-val LEAST_ELIM = store_thm(
-  "LEAST_ELIM",
-  ``!Q P. (?n. P n) /\ (!n. (!m. m < n ==> ~ P m) /\ P n ==> Q n) ==>
-          Q ($LEAST P)``,
-  PROVE_TAC [LEAST_INTRO, LESS_LEAST]);
-
-val LEAST_EXISTS = store_thm
-  ("LEAST_EXISTS",
-   ``!p. (?n. p n) = (p ($LEAST p) /\ !n. n < $LEAST p ==> ~p n)``,
-   GEN_TAC
-   THEN MATCH_MP_TAC EQ_TRANS
-   THEN Q.EXISTS_TAC `?n. p n /\ (!m. m < n ==> ~p m)`
-   THEN CONJ_TAC
-   THENL [(Tactical.REVERSE EQ_TAC THEN1 PROVE_TAC [])
-          THEN REPEAT STRIP_TAC
-          THEN CCONTR_TAC
-          THEN (SUFF_TAC ``!n : num. ~p n`` THEN1 PROVE_TAC [])
-          THEN HO_MATCH_MP_TAC COMPLETE_INDUCTION
-          THEN PROVE_TAC [],
-          (Tactical.REVERSE EQ_TAC THEN1 PROVE_TAC [])
-          THEN STRIP_TAC
-          THEN PROVE_TAC [LESS_LEAST, LEAST_INTRO]]);
-
-val LEAST_EXISTS_IMP = store_thm
-  ("LEAST_EXISTS_IMP",
-   ``!p. (?n. p n) ==> (p ($LEAST p) /\ !n. n < $LEAST p ==> ~p n)``,
-   REWRITE_TAC [LEAST_EXISTS]);
 
 
 val _ = adjoin_to_theory
