src/option/optionScript.sml
@@ -356,6 +356,28 @@ val _ = BasicProvers.export_rewrites
            "OPTION_MAP_DEF", "OPTION_JOIN_DEF", "SOME_11", "NOT_SOME_NONE"]
 
 
+(*---------------------------------------------------------------------------*)
+(* Need to install the constructors for options into the const map.          *)
+(*---------------------------------------------------------------------------*)
+
+val _ = ConstMapML.insert(Term.prim_mk_const{Name="SOME",Thy="option"});
+val _ = ConstMapML.insert(Term.prim_mk_const{Name="NONE",Thy="option"});
+
+val _ = adjoin_to_theory
+{sig_ps = NONE,
+ struct_ps = SOME (fn ppstrm =>
+  let val S = PP.add_string ppstrm
+      fun NL() = PP.add_newline ppstrm
+  in S "val _ = ConstMapML.insert (Term.prim_mk_const{Name=\"SOME\",Thy=\"option\"});";
+     NL(); 
+     S "val _ = ConstMapML.insert (Term.prim_mk_const{Name=\"NONE\",Thy=\"option\"});";
+     NL(); NL()
+  end)}
+
+(*---------------------------------------------------------------------------*)
+(* Export ML versions of option functions                                    *)
+(*---------------------------------------------------------------------------*)
+
 val _ = Drop.exportML("option",
         map Drop.DEFN
          [OPTION_MAP_DEF, IS_SOME_DEF, IS_NONE_DEF, THE_DEF, OPTION_JOIN_DEF]);
